Unified stop parameterized by cause (I)
For a more homogeneous treatment, we return to the original
representation that uses a single constructor for finite traces, and
enrich it with an inductive datatype that represents termination
information, e.g., normal termination, execution error, etc.

As before, we can easily move back and forth between representations
until we need to reason about embeddings and proper prefixes, where
similar issues arise. These are what we need to address next.

TraceModel.v
@@ -7,9 +7,13 @@ Require Import Setoid.
 Require Import List.
 
 (** *traces  *)
+Inductive endstate : Set :=
+| esgood : endstate
+| esbad : endstate
+.
+
 CoInductive trace : Set :=
-  | tstop : trace
-  | tstuck : trace
+  | tstop : endstate -> trace
   | tsilent : trace
   | tcons : event -> trace -> trace.
 
@@ -17,35 +21,25 @@ CoInductive trace : Set :=
 Definition pref := list event.
 
 Inductive finpref : Set :=
-| fstop : pref -> finpref
-| fstuck : pref -> finpref
+| fstop : pref -> endstate -> finpref
 | ftbd  : pref -> finpref
 .
 
-Tactic Notation "destruct" "finpref" ident(m) "as" ident(e) ident(p) :=
-  destruct m as [ [| e p]
-                | [| e p]
+Tactic Notation "destruct" "finpref" ident(m) "as" ident(e) ident(f) ident(p) :=
+  destruct m as [ [| e p] f
                 | [| e p]
                 ].
 
-Tactic Notation "induction" "finpref" ident(m) "as" ident(e) ident(p) ident(Hp) :=
-  destruct m as [m | m | m]; induction m as [|e p Hp].
+Tactic Notation "induction" "finpref" ident(m) "as" ident(e) ident(f) ident(p) ident(Hp) :=
+  destruct m as [m f | m]; induction m as [|e p Hp].
 
 (** *prefix relation *)
-Fixpoint fstop_prefix (m : pref) (t : trace) : Prop :=
+Fixpoint fstop_prefix (m : pref) (f : endstate) (t : trace) : Prop :=
   match m, t with
-    | nil, tstop => True
-    | nil, _     => False
-    | cons e1 m', tcons e2 t' => e1 = e2 /\ fstop_prefix m' t'
-    | _, _       => False
-  end.
-
-Fixpoint fstuck_prefix (m : pref) (t : trace) : Prop :=
-  match m, t with
-    | nil, tstuck => True
-    | nil, _     => False
-    | cons e1 m', tcons e2 t' => e1 = e2 /\ fstuck_prefix m' t'
-    | _, _       => False
+    | nil, tstop f' => f = f'
+    | nil, _        => False
+    | cons e1 m', tcons e2 t' => e1 = e2 /\ fstop_prefix m' f t'
+    | _, _          => False
   end.
 
 Fixpoint ftbd_prefix (m : pref) (t : trace) : Prop :=
@@ -57,8 +51,7 @@ Fixpoint ftbd_prefix (m : pref) (t : trace) : Prop :=
 
 Definition prefix (m : finpref) (t : trace) : Prop :=
   match m with
-  | fstop m => fstop_prefix m t    
-  | fstuck m => fstuck_prefix m t
+  | fstop m f => fstop_prefix m f t
   | ftbd m  => ftbd_prefix m t
   end.
 
@@ -67,8 +60,7 @@ Definition prefix (m : finpref) (t : trace) : Prop :=
 (* fin and inf now refer to *executions*, not traces!
    Eventually they may be given more memorable names than term/nonterm. *)
 Inductive fin : trace -> Prop :=
-  | fin_stop : fin tstop
-  | fin_stuck : fin tstuck
+  | fin_stop : forall f, fin (tstop f)
   | fin_cons : forall e t, fin t -> fin (tcons e t).
 
 Definition inf (t : trace) : Prop := ~(fin t).
@@ -89,11 +81,10 @@ Proof. intros e t H Hc. apply H. now constructor. Qed.
 Lemma many_continuations :
   forall m ta, inf ta -> exists t', prefix m t' /\ t' <> ta.
 Proof.
-  induction finpref m as e m IHm; intros ta Hinf.
-  + exists tstop. split; try now auto.
+  induction finpref m as e f m IHm; intros ta Hinf.
+  + exists (tstop f). split; try now auto.
     intros Hc; subst. apply Hinf. now constructor.
-  + destruct ta as [| | | e' ta].
-    ++ exfalso. apply Hinf. now constructor.
+  + destruct ta as [| | e' ta].
     ++ exfalso. apply Hinf. now constructor.
     ++ specialize (IHm tsilent Hinf).
        destruct IHm as [t' [Hpref Hnsilent]].
@@ -102,22 +93,9 @@ Proof.
        destruct IHm as [t' [Hpref Hneq]]. exists (tcons e t').
        split; try now auto.
        intros Hc. inversion Hc; now subst.
-  + exists tstuck. split; try now auto.
+  + exists (tstop esgood). split; try now auto.
     intros Hc; subst. apply Hinf. now constructor.
-  + destruct ta as [| | | e' ta].
-    ++ exfalso. apply Hinf. now constructor.
-    ++ exfalso. apply Hinf. now constructor.
-    ++ specialize (IHm tsilent Hinf).
-       destruct IHm as [t' [Hpref Hnsilent]].
-       exists (tcons e t'). now split.
-    ++ apply inf_tcons in Hinf. specialize (IHm ta Hinf).
-       destruct IHm as [t' [Hpref Hneq]]. exists (tcons e t').
-       split; try now auto.
-       intros Hc. inversion Hc; now subst.
-  + exists tstop. split; try now auto.
-    intros Hc; subst. apply Hinf. now constructor.
-  + destruct ta as [| | | e' ta].
-    ++ exfalso. apply Hinf. now constructor.
+  + destruct ta as [| | e' ta].
     ++ exfalso. apply Hinf. now constructor.
     ++ specialize (IHm tsilent Hinf).
        destruct IHm as [t' [Hpref Hnsilent]].
@@ -130,17 +108,10 @@ Qed.
 
 (* we try to identify a finite trace and the fpref made of the same events *)
 
-Fixpoint fstop_equal (m : pref) (t : trace) : Prop :=
+Fixpoint fstop_equal (m : pref) (f : endstate) (t : trace) : Prop :=
   match m, t with
-  | nil, tstop => True
-  | cons e1 m', tcons e2 t' => e1 = e2 /\ fstop_equal m' t'
-  | _, _ => False
-  end.
-
-Fixpoint fstuck_equal (m : pref) (t : trace) : Prop :=
-  match m, t with
-  | nil, tstuck => True
-  | cons e1 m', tcons e2 t' => e1 = e2 /\ fstuck_equal m' t'
+  | nil, tstop f' => f = f'
+  | cons e1 m', tcons e2 t' => e1 = e2 /\ fstop_equal m' f t'
   | _, _ => False
   end.
 
@@ -148,41 +119,37 @@ Definition ftbd_equal (m : pref) (t : trace) : Prop := False.
 
 Definition equal (m : finpref) (t : trace) : Prop :=
   match m with
-  | fstop m => fstop_equal m t
-  | fstuck m => fstuck_equal m t
+  | fstop m f => fstop_equal m f t
   | ftbd m  => ftbd_equal m t
   end.
 
 Lemma equal_prefix : forall m t, equal m t -> prefix m t.
 Proof.
-  induction finpref m as e p Hp; destruct t; intros H; now tauto.
+  induction finpref m as e f p Hp; destruct t; intros H; simpl in *; now intuition.
 Qed.
 
 Lemma fin_equal : forall t, fin t <-> exists m : finpref, equal m t.
 Proof.
   intro t. split.
-  - intro H. induction H as [| | e t H [m IH]].
-    + now (exists (fstop nil)).
-    + now (exists (fstuck nil)).
-    + destruct m as [m | m | m].
-      * now (exists (fstop (cons e m))).
-      * now (exists (fstuck (cons e m))).
+  - intro H. induction H as [f | e t H [m IH]].
+    + now (exists (fstop nil f)).
+    + destruct m as [m f | m].
+      * now (exists (fstop (cons e m) f)).
       * now simpl in IH.
   - intros [m Heq]. generalize dependent t.
-    induction finpref m as e m' IH; intros t Heq; try now auto.
+    induction finpref m as e f m' IH; intros t Heq; try now auto.
     + destruct t; try now auto. now constructor.
-    + destruct t as [| | | e' t']; inversion Heq.
-      constructor. now apply IH.
-    + destruct t as [| | | e' t']; inversion Heq.
-      now constructor.
-    + destruct t as [| | | e' t']; inversion Heq.
+    + destruct t as [| | e' t']; inversion Heq.
       constructor. now apply IH.
 Qed.
 
+Print prefix.
 Lemma single_cont : forall m t t', equal m t -> prefix m t' -> t = t'.
 Proof.
-  induction finpref m as e p IHp; destruct t, t'; firstorder;
-  subst; now rewrite (IHp t t').
+  induction finpref m as e f p IHp; destruct t, t'; firstorder;
+  simpl in *; subst.
+  - reflexivity.
+  - now rewrite (IHp t t').
 Qed.
 
 Lemma single_cont_consequence : forall t,
@@ -194,49 +161,48 @@ Qed.
 
 (******************************************************************)
 
+(* RB: For now, we do not care about the type of stop. *)
 Fixpoint fstopped (m : finpref) : bool:=
   match m with
-  | fstop _ => true
-  | fstuck _ => false
+  | fstop _ _ => true
   | ftbd  _ => false
   end. 
 
-Fixpoint fisstuck (m : finpref) : bool:=
-  match m with
-  | fstop _ => false
-  | fstuck _ => true
-  | ftbd  _ => false
-  end. 
+(* Fixpoint fisstuck (m : finpref) : bool:= *)
+(*   match m with *)
+(*   | fstop _ => false *)
+(*   | fstuck _ => true *)
+(*   | ftbd  _ => false *)
+(*   end.  *)
 
 Lemma stop_single_continuation : forall m t1 t2,
     fstopped m = true ->
     prefix m t1 -> prefix m t2 ->
     t1 = t2.
 Proof.
-  intros [m | m | m]; induction m; intros [] [] H H0 H1; try now auto.
+  intros [m | m]; induction m; intros [] [] H H0 H1; try now auto.
+  + simpl in *. now subst.
   + inversion H0. inversion H1. clear H0 H1.
     subst. simpl in H. specialize (IHm t t0 H H3 H5).
     now subst.
 Qed.
 
-(* RB: TODO: Correct name of this lemma later. *)
-Lemma stuck_sngle_continuation : forall m t1 t2,
-    fisstuck m = true ->
-    prefix m t1 -> prefix m t2 ->
-    t1 = t2.
-Proof.
-  intros [m | m | m]; induction m; intros [] [] H H0 H1; try now auto.
-  + inversion H0. inversion H1. clear H0 H1.
-    subst. simpl in H. specialize (IHm t t0 H H3 H5).
-    now subst.
-Qed.
+(* Lemma stuck_sngle_continuation : forall m t1 t2, *)
+(*     fisstuck m = true -> *)
+(*     prefix m t1 -> prefix m t2 -> *)
+(*     t1 = t2. *)
+(* Proof. *)
+(*   intros [m | m | m]; induction m; intros [] [] H H0 H1; try now auto. *)
+(*   + inversion H0. inversion H1. clear H0 H1. *)
+(*     subst. simpl in H. specialize (IHm t t0 H H3 H5). *)
+(*     now subst. *)
+(* Qed. *)
 
-(* RB: TODO: Change name of this lemma later. *)
 Lemma equal_stopped : forall m t,
     equal m t ->
-    fstopped m = true \/ fisstuck m = true.
+    fstopped m = true.
 Proof.
-  intros [m | m | m]; induction m; intros t H;
+  intros [m | m]; induction m; intros t H;
   try now auto.
 Qed.
 
@@ -245,8 +211,7 @@ Qed.
 CoFixpoint constant_trace (e : event) : trace := tcons e (constant_trace e).
 
 Theorem trace_eta : forall t, t = match t with
-                                  | tstop => tstop
-                                  | tstuck => tstuck
+                                  | tstop f => tstop f
                                   | tsilent => tsilent
                                   | tcons e t' => tcons e t'
                                   end.
@@ -271,6 +236,7 @@ Qed.
 CoInductive all (e:event) : trace -> Prop :=
 | acons : forall t, all e t -> all e (tcons e t).
 
+(* RB: This may be extended with the end state later. *)
 Inductive ends_with (e:event) : trace -> Prop :=
 | eall : forall t, all e t -> ends_with e t
 | egrow : forall t e', ends_with e t -> ends_with e (tcons e' t).
@@ -296,7 +262,7 @@ Qed.
    and then add a tstop.
  *)
 
-(* RB: ... *)
+(* RB: What to do with the final state? For now, we leave it as before. *)
 Fixpoint embedding_pref (m : pref) (term : trace) : trace :=
   match m with
   | nil => term
@@ -305,19 +271,18 @@ Fixpoint embedding_pref (m : pref) (term : trace) : trace :=
 
 Definition embedding (m : finpref) : trace :=
   match m with
-  | fstop m => embedding_pref m tstop
-  | fstuck m => embedding_pref m tstuck
-  | ftbd m => embedding_pref m tstop
+  | fstop m f => embedding_pref m (tstop f)
+  | ftbd m => embedding_pref m (tstop esgood) (* RB: The hack. *)
   end.
 
 Lemma embed_pref : forall m, prefix m (embedding m).
-Proof. destruct m as [m | m | m]; now induction m. Qed.
+Proof. destruct m as [m | m]; now induction m. Qed.
 
 Lemma embed_fin : forall m, fin (embedding m).
-Proof. destruct m as [m | m | m]; induction m; now constructor. Qed. 
+Proof. destruct m as [m | m]; induction m; now constructor. Qed. 
 
 Lemma embed_eq : forall m, fstopped m = true -> equal m (embedding m).
-Proof. destruct m as [m | m | m]; induction m; intros H; try now auto.
+Proof. destruct m as [m | m]; induction m; intros H; try now auto.
        simpl in *. now auto.
 Qed.
 
@@ -325,14 +290,11 @@ Lemma equal_embedding : forall m t,
     equal m t ->
     embedding m = t.
 Proof.
-  destruct m as [m | m | m]; induction m; intros t Heq; destruct t; try now auto.
+  destruct m as [m | m]; induction m; intros t Heq; destruct t; try now auto.
+  - inversion Heq. simpl. now subst.
   - inversion Heq. simpl. subst.
-    assert (H: equal (fstop m) t) by auto.
-    assert (H': (embedding (fstop m)) = embedding_pref m tstop) by auto.
-    specialize (IHm t H). now subst.
-  - inversion Heq. simpl. subst.
-    assert (H: equal (fstuck m) t) by auto.
-    assert (H': (embedding (fstuck m)) = embedding_pref m tstuck) by auto.
+    assert (H: equal (fstop m e) t) by auto.
+    assert (H': (embedding (fstop m e)) = embedding_pref m (tstop e)) by auto.
     specialize (IHm t H). now subst.
 Qed.
 
@@ -341,7 +303,6 @@ Lemma embed_cons:  forall m t e,
     (tcons e (embedding m)) = tcons e t.
 Proof.
   intros [] t a He; try now destruct t.
-  simpl in *. now rewrite He.
   simpl in *. now rewrite He.
   simpl in *. now rewrite He.
 Qed.
@@ -370,41 +331,54 @@ Fixpoint fpr_fstop (m1 m2 : pref) : Prop :=
 
 Fixpoint fpr (m1 m2 : finpref) : Prop :=
   match m1, m2 with
-  | ftbd m1, ftbd m2 | ftbd m1, fstop m2 | ftbd m1, fstuck m2 => fpr_ftbd m1 m2
+  | ftbd m1, ftbd m2 | ftbd m1, fstop m2 _ => fpr_ftbd m1 m2
   (* | ftbd m1, fstop m2 => fpr_ftbd m1 m2 *)                                 
-  | fstop m1, fstop m2 | fstuck m1, fstuck m2 => m1 = m2(* or fpr_fstop m1 m2 *)
-  | fstop m1, ftbd m2 | fstuck m1, ftbd m2 | fstop m1, fstuck m2 | fstuck m1, fstop m2 => False
+  | fstop m1 f1, fstop m2 f2 => m1 = m2 /\ f1 = f2 (* or fpr_fstop m1 m2 *)
+  | fstop m1 f1, ftbd m2 => False
   end.
 
 Lemma fpr_reflexivity : forall m, fpr m m.
-Proof.  destruct m as [m | m | m]; now induction m. Qed.
+Proof.  destruct m as [m | m]; now induction m. Qed.
 
 Lemma fpr_transitivity : forall m1 m2 m3,
     fpr m1 m2 -> fpr m2 m3 -> fpr m1 m3.
 Proof.
-  destruct m1 as [m1 | m1 | m1];
-  induction m1; intros [m2 | m2 | m2] [m3 | m3 | m3] H2 H3; auto;
+  destruct m1 as [m1 | m1];
+  induction m1; intros [m2 | m2] [m3 | m3] H2 H3; auto;
   destruct m2; inversion H2; auto;
-    destruct m3; inversion H3; subst; simpl; split; auto.
-  now apply (IHm1 (ftbd m2) (ftbd m3)).
-  now apply (IHm1 (ftbd m2) (ftbd m3)).
-  now apply (IHm1 (ftbd m2) (ftbd m3)).
+    destruct m3; inversion H3; subst; simpl; try discriminate; try split; auto.
+  - inversion H; subst. inversion H1; subst. reflexivity.
+  - inversion H1; subst. reflexivity.
+  - apply (IHm1 (ftbd m2) (ftbd m3)); [easy |].
+    simpl in *. inversion H1; subst. now pose proof fpr_reflexivity (ftbd m3).
+  - now apply (IHm1 (ftbd m2) (ftbd m3)).
+  - now apply (IHm1 (ftbd m2) (ftbd m3)).
 Qed.
 
 Lemma fpr_antisymmetry : forall (m m' : finpref),
     fpr m m' /\ fpr m' m -> m = m'.
 Proof.
   intros m.
-  induction finpref m as e p IHp;
+  induction finpref m as e f p IHp;
     intros m' [H1 H2];
-    destruct finpref m' as e' p';
+    destruct finpref m' as e' f' p';
     try now auto.
+  - inversion H1. now subst.
   - now inversion H1.
   - now inversion H1.
   - specialize (IHp (ftbd p')).
     inversion H1 as [Heq Hpp']; inversion H2 as [_ Hp'p].
     subst.
-    simpl in IHp. assert (H: fpr_ftbd p p' /\ fpr_ftbd p' p) by auto.
+    simpl in IHp. assert (H: fpr_ftbd p p' /\ fpr_ftbd p' p).
+    {
+      inversion Heq; subst.
+      now pose proof fpr_reflexivity (ftbd p').
+    }
+    now inversion Heq.
+  - specialize (IHp (ftbd p')).
+    destruct H1 as [Heq Hpp']; destruct H2 as [_ Hp'p].
+    subst.
+    assert (H: fpr_ftbd p p' /\ fpr_ftbd p' p) by auto.
     specialize (IHp H). now inversion IHp.
 Qed.
 
@@ -412,23 +386,25 @@ Qed.
 Lemma fpr_pref_pref : forall m1 m2 t,
     fpr m1 m2 -> prefix m2 t -> prefix m1 t.
 Proof.
-  destruct m1 as [m1 | m1 | m1].
-  - induction m1; intros [] [] H1 H2; simpl in *; subst; try (now auto).
-  - induction m1; intros [] [] H1 H2; simpl in *; subst; try (now auto).
+  destruct m1 as [m1 | m1].
+  - induction m1; intros [] [] H1 H2;
+      try destruct H1 as [H1 H1']; try destruct H2 as [H2 H2'];
+      simpl in *; subst; try (now auto).
   - induction m1 as [| e m1'].
-    + intros [] [] H1 H2; simpl in *; subst; try (now auto).
+    + intros [] [] H1 H2; simpl in *;
+        try destruct H1 as [H1 H1']; try destruct H2 as [H2 H2'];
+        subst; try (now auto).
     + intros m2 t. intros H1 H2.
-      destruct m2 as [[| e2 m2'] | [| e2 m2'] | [| e2 m2']]; simpl in *; subst; try (now auto);
+      destruct m2 as [[| e2 m2'] f | [| e2 m2']]; simpl in *; subst; try (now auto);
         destruct H1; subst; destruct t; try contradiction;
         destruct H2; subst; split; auto.
-      specialize (IHm1' (fstop m2') t); simpl in *; auto.
-      specialize (IHm1' (fstuck m2') t); simpl in *; auto.
-      specialize (IHm1' (ftbd m2') t); simpl in *; auto.
+      * specialize (IHm1' (fstop m2' f) t); simpl in *; auto.
+      * specialize (IHm1' (ftbd m2') t); simpl in *; auto.
 Qed.
 
 Lemma a_foo_lemma : forall m,
     fpr m (ftbd nil) -> m = ftbd nil.
-Proof. destruct m as [m | m | m]; now induction m. Qed.
+Proof. destruct m as [m | m]; now induction m. Qed.
 
 (* Lemma another_foo_lemma : forall m1 m2 e, *)
 (*     fpr m1 m2 -> fpr (fcons e m1) (fcons e m2). *)
@@ -438,59 +414,37 @@ Lemma same_ext : forall m1 m2 t,
     prefix m1 t -> prefix m2 t ->
     fpr m1 m2 \/ fpr m2 m1.
 Proof.
-  destruct m1 as [m1 | m1 | m1]; induction m1; intros [] [] H1 H2;
+  destruct m1 as [m1 | m1]; induction m1; intros [] [] H1 H2;
     try (now auto); destruct H1; destruct p; simpl in *;
       destruct H2; simpl in *; subst; try (now auto);
-  try (specialize (IHm1 (fstop p) t H0 H2); simpl in IHm1;
-  destruct IHm1; subst; 
+    try specialize (IHm1 _ _ H0);
+    try (specialize (IHm1 (fstop p e0) t H0 H2); simpl in IHm1;
+    destruct IHm1; subst; 
     [now left | now right]);
-  try (specialize (IHm1 (fstuck p) t H0 H2); simpl in IHm1;
-  destruct IHm1; subst; 
-    [now left | now right]);
-  try (specialize (IHm1 (ftbd p) t H0 H2); simpl in IHm1;
-  destruct IHm1; subst; 
-  [now left | now right]).
-Qed.
+    try (specialize (IHm1 (ftbd p) t H0 H2); simpl in IHm1;
+    destruct IHm1; subst; 
+    [now left | now right]).
+(* Qed. *)
+Admitted.
 
 Lemma same_fpr : forall m1 m2 m,
     fpr m1 m -> fpr m2 m ->
     (fpr m1 m2 \/ fpr m2 m1).
 Proof.
-  destruct m1 as [p1 | p1 | p1]; destruct m2 as [p2 | p2 | p2]; destruct m as [p | p | p];
+  destruct m1 as [p1 | p1]; destruct m2 as [p2 | p2]; destruct m as [p | p];
     try now auto.
   - generalize dependent p2. generalize dependent p.
     induction p1.
-    + intros p p2 H1 H2. simpl in *; subst; now left.
-    + intros p p2 H1 H2. simpl in *; subst; now left.
+    + intros p p2 H1 H2; try destruct H1; try destruct H2; simpl in *; subst; now left.
+    + intros p p2 H1 H2; try destruct H1; try destruct H2; simpl in *; subst; now left.
   - generalize dependent p2. generalize dependent p.
     induction p1.
-    + intros p p2 H1 H2. simpl in *; subst; now right.
-    + intros p p2 H1 H2. simpl in *; subst; now right.
+    + intros p p2 H1 H2; try destruct H1; try destruct H2; simpl in *; subst; now right.
+    + intros p p2 H1 H2; try destruct H1; try destruct H2; simpl in *; subst; now right.
   - generalize dependent p2. generalize dependent p.
     induction p1.
-    + intros p p2 H1 H2. simpl in *; subst; now left.
-    + intros p p2 H1 H2. simpl in *; subst; now left.
-  - generalize dependent p2. generalize dependent p.
-    induction p1.
-    + intros p p2 H1 H2. simpl in *; subst; now right.
-    + intros p p2 H1 H2. simpl in *; subst; now right.
-  - generalize dependent p2. generalize dependent p.
-    induction p1.
-    + intros p p2 H1 H2. simpl in *; subst; now left.
-    + intros p p2 H1 H2. simpl in *; subst; now left.
-  - generalize dependent p2. generalize dependent p.
-    induction p1.
-    + intros p p2 H1 H2. simpl in *; subst; now left.
-    + intros p p2 H1 H2. simpl in *; subst; now left.
-  - generalize dependent p2. generalize dependent p.
-    induction p1.
-    + intros p p2 H1 H2. simpl in *; subst; now left.
-    + intros p p2 H1 H2. simpl in *; subst.
-      destruct p as [| a' p'].
-      ++ contradiction.
-      ++ destruct H1; subst. destruct p2; auto.
-         simpl in H2; destruct H2; subst. specialize (IHp1 p' p2 H0 H1).
-         destruct IHp1; [now left | now right].
+    + intros p p2 H1 H2; try destruct H1; try destruct H2; simpl in *; subst; now left.
+    + intros p p2 H1 H2; try destruct H1; try destruct H2; simpl in *; subst; now left.
   - generalize dependent p2. generalize dependent p.
     induction p1.
     + intros p p2 H1 H2. simpl in *; subst; now left.
@@ -520,16 +474,19 @@ Proof.
 Qed.
 
 Lemma no_prper_fpr_ftbd : forall m, m <> ftbd nil -> fpr m (ftbd nil) -> False.
-Proof. destruct m as [m | m | m]; now induction m. Qed.
+Proof. destruct m as [m | m]; now induction m. Qed.
 
 Lemma stop_sngle_continuation_fpr : forall m1 m2,
     fstopped m1 = true ->
     fpr m1 m2 ->
     m1 = m2.
 Proof.
-  destruct m1 as [m1 | m1 | m1]; destruct m2 as [m2 | m2 | m2];
-    induction m1, m2; try now auto.
-  intros H H0; simpl in *; subst. now rewrite H0.
+  destruct m1 as [m1 | m1]; destruct m2 as [m2 | m2];
+    induction m1, m2;
+    intros H H0;
+    inversion H0; subst;
+    try now auto.
+  - congruence.
 Qed.
 
 (**************************************************)
@@ -546,8 +503,7 @@ Fixpoint snoc {A : Type} (l : list A) (x : A) : list A :=
 
 Definition fsnoc (m : finpref) (e : event) :=
   match m with
-  | fstop m' => m
-  | fstuck m' => m
+  | fstop m' _ => m
   | ftbd  m' => ftbd (snoc m' e)
   end.
 
@@ -562,11 +518,11 @@ Lemma fpr_snoc_fpr : forall m1 m2 e,
     fpr m1 m2 ->
     fpr m1 (fsnoc m2 e).
 Proof.
-  destruct m1 as [m1 | m1 | m1]; induction m1; intros [] e H; try now auto;
+  destruct m1 as [m1 | m1]; induction m1; intros [] e' H; try now auto;
   inversion H; subst.
   + simpl in *. destruct p. contradiction.
     destruct H as [H1 H2].
-    specialize (IHm1 (ftbd p) e H2). now split.
+    specialize (IHm1 (ftbd p) e' H2). now split.
 Qed.
 
 Lemma snoc_stop' : forall m e b, fstopped (fsnoc m e) = b ->
@@ -592,7 +548,7 @@ Lemma compare_with_snoc : forall m1 m e,
     fpr m1 (fsnoc m e) ->
     (fpr m1 m \/ m1 = fsnoc m e).
 Proof.
-  destruct m1 as [m1 | m1 | m1]; induction m1; destruct m as [m | m | m];
+  destruct m1 as [m1 | m1]; induction m1; destruct m as [m | m];
     induction m; intros e' H; try now auto.
   + inversion H. assert (fpr (ftbd m1) (ftbd nil)).
     { auto. }
@@ -607,11 +563,10 @@ Qed.
 
 Lemma snoc_diff : forall m a b,
     fstopped m = false ->
-    fisstuck m = false ->
     fpr (fsnoc m a) (fsnoc m b) ->
     a = b.
 Proof.
-  intros [m|m|m] a b H H' H0; [now inversion H | now inversion H' |].
+  intros [m|m] a b H H0; [now inversion H |].
   clear H. simpl in *.
   eapply (compare_with_snoc (fsnoc (ftbd m) a) (ftbd m) b) in H0.
   destruct H0 as [H0 | H0]; auto.
@@ -623,21 +578,20 @@ Proof.
 Qed.
 
 Lemma no_snoc_fpr_ftb : forall m e, ~ fpr (fsnoc m e) (ftbd nil).
-Proof. destruct m as [m | m | m]; now induction m. Qed.
+Proof. destruct m as [m | m]; now induction m. Qed.
 
 Lemma fpr_snoc_ftbd : forall m e f,
     fstopped m = false ->
-    fisstuck m = false ->
     fpr (fsnoc m e) (fsnoc (ftbd nil) f) ->
     m = ftbd nil.
 Proof.
-  intros [m|m|m] e f H H' H0; [now induction m | now induction m |].
+  intros [m|m] e' f H H0; [now induction m |].
   + apply compare_with_snoc in H0. destruct H0.
     now apply no_snoc_fpr_ftb in H0.
     simpl in H0. inversion H0.
     destruct m; auto.
     simpl in *. clear H. inversion H2. subst.
-    assert (H: ~ (snoc m e = nil)).
+    assert (H: ~ (snoc m e' = nil)).
     { now induction m. }
     contradiction.
 Qed.
@@ -646,79 +600,68 @@ Lemma same_snoc_same_finpref : forall m m0 e1 e2 i1 i2,
     i1 <> i2  -> e1 <> e2 ->
     fstopped m0 = false ->
     fstopped m = false ->
-    fisstuck m0 = false ->
-    fisstuck m = false ->
     fpr (fsnoc m0 i1) (fsnoc m e1) ->
     fpr (fsnoc m0 i2) (fsnoc m e2) ->
     m0 = m.
 Proof.
-  destruct m as [m | m | m]; induction m as [| e' m' IHm'];
-  intros m0 e1 e2 i1 i2 H H0 H' H0' H1 H2 H3 H4;
+  destruct m as [m | m]; induction m as [| e' m' IHm'];
+  intros m0 e1 e2 i1 i2 H H0 H1 H2 H3 H4;
   try now auto; simpl in *.
   + now apply (fpr_snoc_ftbd m0 i1 e1).
-  + destruct m0 as [m0 | m0 | m0];
-    [now inversion H1 | now inversion H1 |].
+  + destruct m0 as [m0 | m0];
+    [now inversion H1 |].
     destruct m0 as [| e0 m0]; simpl in *. destruct H3, H4; subst; contradiction.
     destruct H3, H4; subst.
-    specialize (IHm' (ftbd m0) e1 e2 i1 i2 H H0 H1 H2 H' H0' H5 H6). now inversion IHm'.
+    specialize (IHm' (ftbd m0) e1 e2 i1 i2 H H0 H1 H2 H5 H6). now inversion IHm'.
 Qed.
 
 Lemma snoc_lemma : forall m,
     m = ftbd nil \/
     (exists m' e', m = fsnoc m' e').
 Proof.
-  intros [m | m | m]; induction m.
-  - right. now exists (fstop nil), an_event.
+  intros [m f | m]; induction m.
+  - right. now exists (fstop nil f), an_event.
   - destruct IHm as [H | H]; try now inversion H.
-    right. destruct H as [m' [e' H]]. now exists (fstop (cons a m)), e'.
-  - right. now exists (fstuck nil), an_event.
-  - destruct IHm as [H | H]; try now inversion H.
-    right. destruct H as [m' [e' H]]. now exists (fstuck (cons a m)), e'.
+    right. destruct H as [m' [e' H]]. now exists (fstop (cons a m) f), e'.
   - now left.
   - destruct IHm as [H | H]. 
     + inversion H; subst. right. now exists (ftbd nil), a.
     + destruct H as [m' [e' H]]. right.
-      destruct m' as [m' | m' | m'].
-      now exists (ftbd (cons a m')), e'.
+      destruct m' as [m' | m'].
       now exists (ftbd (cons a m')), e'.
       inversion H. exists (ftbd (cons a m')), e'. now subst. 
 Qed.
 
 Lemma not_stop_not_snoc_pref : forall m e,
     fstopped m = false ->
-    fisstuck m = false ->
     fpr (fsnoc m e) m -> False.
 Proof.
-  intros [m | m | m] e H H0; induction m; try now auto.
+  intros [m f | m] e H H0; induction m; try now auto.
   simpl in *. destruct H0 as [Heq H0].
-  intros [H1 H2].
   apply IHm; try reflexivity. assumption.
 Qed.
 
 Lemma snoc_m_event_equal : forall m e1 e2,
     fstopped m = false ->
-    fisstuck m = false ->
     fpr (fsnoc m e1) (fsnoc m e2) ->
     e1 = e2.
 Proof.
-  intros [m | m | m] e1 e2 Hstop Hstuck Hfpr;
+  intros [m f | m] e1 e2 Hstop Hfpr;
   induction m; inversion Hfpr; try now auto.
 Qed.
 
 Lemma same_snoc_same_pointwise : forall m1 m2 e1 e2,
     fstopped m1 = false ->
     fstopped m2 = false ->
-    fisstuck m1 = false ->
-    fisstuck m2 = false ->
     fsnoc m1 e1 = fsnoc m2 e2 ->
     m1 = m2 /\ e1 = e2.
 Proof.
-  destruct m1 as [m1 | m1 | m1]; induction m1; intros m2 e1 e2 Hstop1 Hstop2 Hstuck1 Hstuck2 Heq;
+  destruct m1 as [m1 | m1]; induction m1; intros m2 e1 e2 Hstop1 Hstop2 Heq;
     try now auto.
-  + destruct m2 as [m2 | m2 | m2]; destruct m2; inversion Heq; try now auto.
+  + destruct m2 as [m2 | m2]; destruct m2; inversion Heq; try now auto.
     simpl in *. 
     ++ now destruct m2. 
-  + destruct m2 as [m2 | m2 | m2]; destruct m2; inversion Heq; try now auto.
+  + destruct m2 as [m2 | m2]; destruct m2; inversion Heq; try now auto.
     ++ exfalso. apply (no_snoc_fpr_ftb (ftbd m1) e1). simpl in *. now rewrite H1. 
     ++ destruct (IHm1 (ftbd m2) e1 e2); simpl in *; subst; try now auto.
        now rewrite H1. inversion H; now subst.
